ironfleet/src/Dafny/Distributed/Concur/ReductionBasic.i.dfy
@@ -39,4 +39,34 @@ module ReductionBasicModule
             new_pivot_index := pivot_index - 1;
         }
     }
+
+    lemma lemma_IfTreeHasNoChildrenThenItHasNoLeafEntries(tree:Tree)
+        requires tree.Inner?;
+        requires |tree.children| == 0;
+        ensures  |GetLeafEntries(tree)| == 0;
+    {
+    }
+
+    lemma lemma_IfAllRootsAreLeavesThenGetLeafEntriesForestAreRoots(trees:seq<Tree>)
+        requires forall tree :: tree in trees ==> tree.Leaf?;
+        ensures  |GetLeafEntriesForest(trees)| == |trees|;
+        ensures  forall i {:trigger trees[i]}{:trigger GetLeafEntriesForest(trees)[i]} ::
+                      0 <= i < |trees| ==> GetLeafEntriesForest(trees)[i] == trees[i].entry;
+    {
+        if |trees| == 0 {
+            return;
+        }
+
+        lemma_IfAllRootsAreLeavesThenGetLeafEntriesForestAreRoots(trees[1..]);
+    }
+
+    lemma lemma_IfAllChildrenAreLeavesThenGetLeafEntriesAreChildren(tree:Tree)
+        requires tree.Inner?;
+        requires forall c :: c in tree.children ==> c.Leaf?;
+        ensures  |tree.children| == |GetLeafEntries(tree)|;
+        ensures  forall i {:trigger GetLeafEntries(tree)[i]}{:trigger tree.children[i]} ::
+                      0 <= i < |tree.children| ==> GetLeafEntries(tree)[i] == tree.children[i].entry;
+    {
+        lemma_IfAllRootsAreLeavesThenGetLeafEntriesForestAreRoots(tree.children);
+    }
 }
